coq/verif_map.v
@@ -11,9 +11,9 @@ Local Open Scope Z.
 Inductive repr : Z -> val -> Prop :=
 | mk_repr : forall z, Int.min_signed <= z <= Int.max_signed -> repr z (Vint (Int.repr z)).
 
-Inductive Irepr : nat -> val -> Prop :=
-| mk_Irepr : forall i:nat, (0 <= i <= Z.to_nat(Int.max_signed))%nat ->
-                           Irepr i (Vint (Int.repr (Z.of_nat i))).
+Inductive Nrepr : nat -> val -> Prop :=
+| mk_Nrepr : forall i:nat, (0 <= i <= Z.to_nat(Int.max_signed))%nat ->
+                           Nrepr i (Vint (Int.repr (Z.of_nat i))).
 
 (* Function specifications *)
 Definition loop_spec :=
@@ -30,8 +30,9 @@ Definition find_empty_spec :=
     WITH sh : share, m : ArrMapZ, start : Z, i : nat,
          vbb : val, vstart : val, vi : val
     PRE [_busybits OF (tptr tint), _start OF tint, _i OF tint]
-        PROP (0 <= start < 100; repr start vstart; Irepr i vi;
-              isptr vbb)
+        PROP (0 <= start < 100;
+              repr start vstart; Nrepr i vi; isptr vbb;
+              (Z.of_nat i < 261905)(*my max recursion depth*))
         LOCAL (`(eq vstart) (eval_id _start);
                `(eq vi) (eval_id _i);
                `(eq vbb) (eval_id _busybits))
@@ -86,8 +87,10 @@ Definition find_key_spec :=
          vbb : val, vkeys : val, vstart : val, vkey : val, vi : val
     PRE [_busybits OF (tptr tint), _keys OF (tptr tint),
          _start OF tint, _key OF tint, _i OF tint]
-        PROP (0 <= start < 100; repr start vstart; repr key vkey;
-              Irepr i vi; isptr vbb; isptr vkeys)
+        PROP (0 <= start < 100;
+              repr start vstart;
+              repr key vkey; Nrepr i vi; isptr vbb; isptr vkeys;
+              (Z.of_nat i < 261905)(*my max recursion depth*))
         LOCAL (`(eq vstart) (eval_id _start);
                `(eq vkey) (eval_id _key);
                `(eq vi) (eval_id _i);
@@ -229,7 +232,11 @@ Ltac get_repr k :=
       |[H:?a = (Int.repr k)|-context[Int.signed ?a]] =>
        rewrite H; rewrite Int.signed_repr;[|repr_bound k]
       |[H:?a = (Int.repr k)|-context[?a]] => rewrite H
-      |[H:?a = (Vint (Int.repr k))|-context[?a]] => rewrite H; idtac "ololo"
+      |[H:?a = (Vint (Int.repr k))|-context[?a]] => rewrite H
+      |[H:?a = (Int.repr Z.of_nat(k))|-context[Int.signed ?a]] =>
+       rewrite H; rewrite Int.signed_repr;[|repr_bound k]
+      |[H:?a = (Int.repr (Z.of_nat k))|-context[?a]] => rewrite H
+      |[H:?a = (Vint (Int.repr (Z.of_nat k)))|-context[?a]] => rewrite H
       |[H:k = ?a|-context[?a]]=>rewrite <- H
       |[H:repr k (Vint ?a) |-context[?a]] =>
        let H' := fresh a "EQ" k in
@@ -237,6 +244,16 @@ Ltac get_repr k :=
       |[H:repr k ?a |-context[?a]] =>
        let H' := fresh "EQ" k in
        assert (a = (Vint (Int.repr k))) as H' by (inv H; tauto)
+      |[H1:repr k ?a, H2:?a = Vint ?b |-context[?b]] =>
+       let H' := fresh "EQ" k in
+       assert (a = (Vint (Int.repr k))) as H' by (inv H1; tauto);
+         let Hinj := fresh "EQ" b in
+         rewrite H' in H2; injection H2 as Hinj; symmetry in Hinj
+      |[H1:Nrepr k ?a, H2:?a = Vint ?b |-context[?b]] =>
+       let H' := fresh "EQ" k in
+       assert (a = (Vint (Int.repr (Z.of_nat k)))) as H' by (inv H1; tauto);
+         let Hinj := fresh "EQ" b in
+         rewrite H' in H2; injection H2 as Hinj; symmetry in Hinj
     end.
 
 (* Auxillary lemmas *)
@@ -295,4 +312,128 @@ Proof.
           omega.
       }
       unfold_to_bare_Z.
+Qed.
+
+Lemma body_find_empty: semax_body Vprog Gprog f_find_empty find_empty_spec.
+Proof.
+  start_function.
+  name bbarg _busybits.
+  name sarg _start.
+  name iarg _i.
+  name indexloc _index.
+  name bbloc _bb.
+  forward_call (sh,(start + Z.of_nat i + 1), (* loop(1 + start + i) *)
+                (Vint (Int.repr (start + Z.of_nat i + 1)))).
+  entailer!.
+  - constructor.
+    unfold_to_bare_Z.
+  - get_repr start.
+    get_repr i.
+    unfold_to_bare_Z.
+    apply f_equal;omega.
+  - auto with closed.
+  - after_call.
+    forward.
+    pose (Loop_bound (start + Z.of_nat i + 1)).
+    entailer!.
+    apply Loop_bound.
+    simpl;auto.
+    forward_if (PROP (busybits m (loop (start + Z.of_nat i + 1)) = true)
+                LOCAL (`(eq vi) (eval_id _i);
+                       `(eq vstart) (eval_id _start);
+                       `(eq vbb) (eval_id _busybits))
+                SEP(`(array_at tint sh (fun x =>
+                                    (Vint (Int.repr (if (busybits m x)
+                                                     then 1
+                                                     else 0))))
+                         0 100 vbb))).
+    + pose (Loop_bound (start + Z.of_nat i + 1)).
+      forward. entailer!.
+      unfold find_empty.
+      rewrite find_if_equation.
+      rewrite Int.signed_repr in H4.
+      assert ( busybits m (loop (1 + start + Z.of_nat i)) = false) as REWR. {
+        replace (1 + start + Z.of_nat i) with (start + Z.of_nat i + 1);[|omega].
+        destruct ( busybits m (loop (start + Z.of_nat i + 1))).
+        apply int_eq_e in H4.
+        discriminate H4.
+        tauto.
+      }
+      rewrite REWR.
+      replace (1 + start + Z.of_nat i) with (start + Z.of_nat i + 1);[|omega].
+      simpl.
+      tauto.
+      unfold_to_bare_Z.
+    + forward.
+      entailer!.
+      rewrite Int.signed_repr in H4.
+      destruct ( busybits m (loop (start + Z.of_nat i + 1))).
+      tauto.
+      rewrite Int.eq_true in H4.
+      discriminate H4.
+      pose (Loop_bound (start + Z.of_nat i + 1));unfold_to_bare_Z.
+    + forward_if (PROP((0 < i)%nat;
+                       busybits m (loop (start + Z.of_nat i + 1)) = true)
+                  LOCAL(`(eq vi) (eval_id _i);
+                        `(eq vstart) (eval_id _start);
+                        `(eq vbb) (eval_id _busybits))
+                  SEP(`(array_at tint sh (fun x =>
+                                            (Vint (Int.repr (if (busybits m x)
+                                                             then 1
+                                                             else 0))))
+                                 0 100 vbb))).
+      forward. entailer!.
+      * replace (start + Z.of_nat i + 1) with (1 + start + Z.of_nat i) in H4;[|omega].
+        assert (i = 0)%nat. {
+        admit.
+        }
+        subst i.
+        unfold find_empty.
+        rewrite find_if_equation.
+        rewrite H4.
+        auto_logic.
+      * forward.
+        entailer!.
+        assert (i <> 0)%nat by admit.
+        omega.
+      * {forward_call(sh, m, start, (i - 1)%nat, vbb, vstart,
+                     (Vint (Int.repr (Z.of_nat (i - 1))))).
+         entailer!.
+         - rewrite <- H8.
+           assumption.
+         - constructor.
+           try omega.
+           split.
+           omega.
+           apply Nat2Z.inj_le.
+           rewrite Nat2Z.inj_sub.
+           rewrite Z2Nat.id.
+           simpl.
+           unfold_int_limits.
+           omega.
+           unfold_int_limits;omega.
+           omega.
+         - rewrite Nat2Z.inj_sub.
+           omega.
+           omega.
+         - get_repr i.
+           rewrite sub_repr.
+           rewrite Nat2Z.inj_sub.
+           simpl.
+           tauto.
+           omega.
+         - after_call.
+           forward.
+           entailer!.
+           unfold find_empty.
+           rewrite find_if_equation.
+           replace (start + Z.of_nat i + 1) with (1 + start + Z.of_nat i) in H5;[|omega].
+           rewrite H5.
+           simpl.
+           destruct i.
+           omega.
+           unfold find_empty in H6.
+           replace (S i - 1)%nat with i in H6;[|omega].
+           assumption.
+        }
 Qed.
